move most of ML to THY Note: the priority type is defined with 'nat' instead of 'int'.
git-svn-id: https://projects.brucker.ch/hol-testgen/svn/HOL-TestGen/trunk/hol-testgen@9840 3260e6d1-4efc-4170-b0a7-36055960796d

src/OCL_class_diagram_generator.thy
@@ -3,7 +3,7 @@
  *                       for the OMG Standard.
  *                       http://www.brucker.ch/projects/hol-testgen/
  *
- * OCL_class_diagram_generator.thy --- 
+ * OCL_class_diagram_generator.thy ---
  * This file is part of HOL-TestGen.
  *
  * Copyright (c) 2013      Universite Paris-Sud, France
@@ -47,7 +47,7 @@ theory OCL_class_diagram_generator
 imports Main
 begin
 
-definition "bug_ocaml_extraction = id" 
+definition "bug_ocaml_extraction = id"
   (* In this theory, this identifier can be removed everywhere it is used.
      However without this, there is a syntax error when the code is extracted to OCaml. *)
 
@@ -94,11 +94,11 @@ datatype simplety = Opt str | Raw str
 datatype dataty = Datatype str (* name *)
                            "(str (* name *) \<times> simplety list (* arguments *)) list" (* constructors *)
 
-datatype raw_ty = 
+datatype raw_ty =
    Ty_apply raw_ty "raw_ty list"
  | Ty_base str
 
-datatype ty_synonym = Type_synonym str (* name *) 
+datatype ty_synonym = Type_synonym str (* name *)
                                    raw_ty (* content *)
 
 datatype expr = Expr_case expr (* value *)
@@ -117,14 +117,14 @@ datatype expr = Expr_case expr (* value *)
 
 datatype instantiation_class = Instantiation str (* name *)
                                              str (* name in definition *)
-                                             expr 
+                                             expr
 
 datatype defs_overloaded = Defs_overloaded str (* name *) expr (* content *)
 
 datatype consts_class = Consts str (* name *) str (* type output *) str (* ocl symbol1 *) str (* ocl symbol2 *)
 
 datatype definition_hol = Definition expr
-                        | Definition_abbrev str (* name *) "expr (* syntax extension *) \<times> int (* priority *)" expr
+                        | Definition_abbrev str (* name *) "expr (* syntax extension *) \<times> nat (* priority *)" expr
 
 datatype lemmas_simp = Lemmas_simp "str list"
 
@@ -183,7 +183,7 @@ definition "var_select = ''select''"
 section{* Model of OCL classes *}
 
 fun map_class_gen where
-   "map_class_gen f (Mk_univ name l_attr dataty) = 
+   "map_class_gen f (Mk_univ name l_attr dataty) =
   ((case dataty of None \<Rightarrow> [] | Some dataty \<Rightarrow> map_class_gen f dataty) @
    f (\<lambda>s. s @ isub_of_str name) name l_attr)"
 
@@ -201,7 +201,7 @@ subsection{* ... *}
 fun print_datatype_class where
    "print_datatype_class (Mk_univ name l_attr dataty) =
   (let (l_cons, v) = (case dataty of None \<Rightarrow> ([],[]) | Some dataty \<Rightarrow> print_datatype_class dataty) in
-   (name # l_cons, 
+   (name # l_cons,
     v @
     (let isub_name = (\<lambda>s. s @ isub_of_str name) in
     [ Datatype
@@ -213,12 +213,12 @@ fun print_datatype_class where
         [ (isub_name datatype_constr_name, [ bug_ocaml_extraction (Raw (str_of_ty object))
                                            , Raw (isub_name datatype_ext_name) ] ) ] ])))"
 
-definition "print_datatype_universe = 
+definition "print_datatype_universe =
   map_class (\<lambda>isub_name _ _. (isub_name datatype_in, [Raw (isub_name datatype_name)]))"
 
 definition "print_type_synonym_class =
   map_class (\<lambda>isub_name name _.
-    Type_synonym name (Ty_apply (Ty_base ''val'') [Ty_base unicode_AA, 
+    Type_synonym name (Ty_apply (Ty_base ''val'') [Ty_base unicode_AA,
     let option = (\<lambda>x. Ty_apply (Ty_base ''option'') [x]) in
     option (option (Ty_base (isub_name datatype_name))) ]))"
 
@@ -261,28 +261,28 @@ definition "print_astype_consts =
     Consts (isub_name const_oclastype) name dot_oclastype name)"
 
 definition "print_astype_from_universe =
-  map_class_h (\<lambda>isub_name name l_hierarchy. 
+  map_class_h (\<lambda>isub_name name l_hierarchy.
     let const_astype = concat (const_oclastype # isub_of_str name # ''_'' # unicode_AA # [])
       ; var_u = ''u'' in
-    Definition (Expr_rewrite (Expr_basic [const_astype]) ''='' (Expr_lambda var_u 
+    Definition (Expr_rewrite (Expr_basic [const_astype]) ''='' (Expr_lambda var_u
 
-   (let ((finish_with_some1, finish_with_some2), last_case_none) = 
+   (let ((finish_with_some1, finish_with_some2), last_case_none) =
      let (f, r) = (if hd l_hierarchy = name then (id, []) else (flip, [(Expr_basic [wildcard], Expr_basic [''None''])])) in
      (f (id, Expr_some), r) in
    finish_with_some2
-   (Expr_case (Expr_basic [var_u]) (concat (map 
-   (\<lambda>h_name. 
+   (Expr_case (Expr_basic [var_u]) (concat (map
+   (\<lambda>h_name.
      let isub_h = (\<lambda> s. s @ isub_of_str h_name)
        ; var_oid = ''oid''
-       ; pattern_complex = (\<lambda>h_name name. 
+       ; pattern_complex = (\<lambda>h_name name.
                             let isub_h = (\<lambda> s. s @ isub_of_str h_name)
-                              ; isub_name = (\<lambda>s. s @ isub_of_str name) 
+                              ; isub_name = (\<lambda>s. s @ isub_of_str name)
                               ; isub_n = (\<lambda>s. isub_name (concat (s # ''_'' # [])))
                               ; var_name = name in
-                             Expr_apply (isub_h datatype_constr_name) 
+                             Expr_apply (isub_h datatype_constr_name)
                                         [Expr_basic [var_oid], Expr_apply (isub_n (isub_h datatype_ext_constr_name)) [Expr_basic [var_name]]])
        ; pattern_simple = (\<lambda> name.
-                            let isub_name = (\<lambda>s. s @ isub_of_str name) 
+                            let isub_name = (\<lambda>s. s @ isub_of_str name)
                               ; var_name = name in
                              Expr_basic [isub_name datatype_constr_name, var_oid, var_name])
        ; case_branch = (\<lambda>pat res. (Expr_apply (isub_h datatype_in) [pat], finish_with_some1 res)) in
@@ -296,39 +296,39 @@ definition "print_astype_class =
   map_class_gen_h (\<lambda>isub_name name l_hierarchy.
     map
       (\<lambda> h_name.
-        Defs_overloaded 
+        Defs_overloaded
           (concat (isub_name const_oclastype # ''_'' # h_name # []))
           (let var_x = ''x'' in
            Expr_rewrite
              (Expr_postunary (Expr_annot (Expr_basic [var_x]) h_name) (Expr_basic [dot_astype name]))
              unicode_equiv
-             (let x = compare_hierarchy l_hierarchy h_name name in 
+             (let x = compare_hierarchy l_hierarchy h_name name in
               if x = Some EQ then
                 Expr_basic [var_x]
               else
                 let var_tau = unicode_tau
                   ; val_invalid = Expr_apply ''invalid'' [Expr_basic [var_tau]] in
-                Expr_lambda var_tau 
+                Expr_lambda var_tau
                   (Expr_case
                     (Expr_apply var_x [Expr_basic [var_tau]])
                     ( (Expr_basic [unicode_bottom], val_invalid)
                     # (Expr_some (Expr_basic [unicode_bottom]), Expr_apply ''null'' [Expr_basic [var_tau]])
                     # (let var_oid = ''oid''
-                         ; pattern_complex = (\<lambda>h_name name. 
+                         ; pattern_complex = (\<lambda>h_name name.
                             let isub_h = (\<lambda> s. s @ isub_of_str h_name)
-                              ; isub_name = (\<lambda>s. s @ isub_of_str name) 
+                              ; isub_name = (\<lambda>s. s @ isub_of_str name)
                               ; isub_n = (\<lambda>s. isub_name (concat (s # ''_'' # [])))
                               ; var_name = name in
-                             Expr_apply (isub_h datatype_constr_name) 
+                             Expr_apply (isub_h datatype_constr_name)
                                         [Expr_basic [var_oid], Expr_apply (isub_n (isub_h datatype_ext_constr_name)) [Expr_basic [var_name]]])
                          ; pattern_simple = (\<lambda> name.
-                            let isub_name = (\<lambda>s. s @ isub_of_str name) 
+                            let isub_name = (\<lambda>s. s @ isub_of_str name)
                               ; var_name = name in
                              Expr_basic [isub_name datatype_constr_name, var_oid, var_name])
                          ; some_some = (\<lambda>x. Expr_some (Expr_some x)) in
                        if x = Some LT then
                          [ (some_some (pattern_simple h_name), some_some (pattern_complex name h_name)) ]
-                       else 
+                       else
                          [ (some_some (pattern_complex h_name name), some_some (pattern_simple name))
                          , (Expr_basic [wildcard], val_invalid) ]) ) ))) )
       l_hierarchy)"
@@ -340,7 +340,7 @@ definition "print_astype_lemmas_id =
 definition "print_astype_lemma_cp =
   get_hierarchy (\<lambda>l_hierarchy.
   concat (concat
-  (map (\<lambda>name1. map (\<lambda>name2. map (\<lambda>name3. 
+  (map (\<lambda>name1. map (\<lambda>name2. map (\<lambda>name3.
     Lemma_by
       (concat (''cp_'' # const_oclastype # isub_of_str name1 # ''_'' # name3 # ''_'' # name2 # []))
       (bug_ocaml_extraction (let var_p = ''p''; var_x = ''x'' in
@@ -359,14 +359,14 @@ definition "print_astype_lemmas_cp =
   get_hierarchy (\<lambda>l_hierarchy.
     [Lemmas_simp
       (concat (concat
-        (map (\<lambda>name1. map (\<lambda>name2. map (\<lambda>name3. 
+        (map (\<lambda>name1. map (\<lambda>name2. map (\<lambda>name3.
           (concat (''cp_'' # const_oclastype # isub_of_str name1 # ''_'' # name3 # ''_'' # name2 # []))
         ) l_hierarchy) l_hierarchy) l_hierarchy)))])"
 
-definition "print_astype_lemma_strict = 
+definition "print_astype_lemma_strict =
   get_hierarchy (\<lambda>l_hierarchy.
   concat (concat
-  (map (\<lambda>name1. map (\<lambda>name2. map (\<lambda>name3. 
+  (map (\<lambda>name1. map (\<lambda>name2. map (\<lambda>name3.
     Lemma_by
       (concat (const_oclastype # isub_of_str name1 # ''_'' # name3 # ''_'' # name2 # []))
       [ Expr_rewrite
@@ -386,7 +386,7 @@ definition "print_astype_lemmas_strict =
   get_hierarchy (\<lambda>l_hierarchy.
   [ Lemmas_simp
       (concat (concat
-      (map (\<lambda>name1. map (\<lambda>name2. map (\<lambda>name3. 
+      (map (\<lambda>name1. map (\<lambda>name2. map (\<lambda>name3.
         (concat (const_oclastype # isub_of_str name1 # ''_'' # name3 # ''_'' # name2 # []))
       ) l_hierarchy) [''invalid'',''null'']) l_hierarchy)))])"
 
@@ -397,28 +397,28 @@ definition "print_istypeof_consts =
     Consts (isub_name const_oclistypeof) ty_boolean dot_oclistypeof name)"
 
 definition "print_istypeof_from_universe =
-  map_class_h (\<lambda>isub_name name l_hierarchy. 
+  map_class_h (\<lambda>isub_name name l_hierarchy.
     let const_istypeof = concat (const_oclistypeof # isub_of_str name # ''_'' # unicode_AA # [])
       ; var_u = ''u'' in
-    Definition (Expr_rewrite (Expr_basic [const_istypeof]) ''='' (Expr_lambda var_u 
+    Definition (Expr_rewrite (Expr_basic [const_istypeof]) ''='' (Expr_lambda var_u
 
-   (let ((finish_with_some1, finish_with_some2), last_case_none) = 
+   (let ((finish_with_some1, finish_with_some2), last_case_none) =
      let (f, r) = (if hd l_hierarchy = name then (id, []) else (flip, [(Expr_basic [wildcard], Expr_basic [''None''])])) in
      (f (id, Expr_some), r) in
    finish_with_some2
-   (Expr_case (Expr_basic [var_u]) (concat (map 
-   (\<lambda>h_name. 
+   (Expr_case (Expr_basic [var_u]) (concat (map
+   (\<lambda>h_name.
      let isub_h = (\<lambda> s. s @ isub_of_str h_name)
        ; var_oid = ''oid''
-       ; pattern_complex = (\<lambda>h_name name. 
+       ; pattern_complex = (\<lambda>h_name name.
                             let isub_h = (\<lambda> s. s @ isub_of_str h_name)
-                              ; isub_name = (\<lambda>s. s @ isub_of_str name) 
+                              ; isub_name = (\<lambda>s. s @ isub_of_str name)
                               ; isub_n = (\<lambda>s. isub_name (concat (s # ''_'' # [])))
                               ; var_name = name in
-                             Expr_apply (isub_h datatype_constr_name) 
+                             Expr_apply (isub_h datatype_constr_name)
                                         [Expr_basic [var_oid], Expr_apply (isub_n (isub_h datatype_ext_constr_name)) [Expr_basic [var_name]]])
        ; pattern_simple = (\<lambda> name.
-                            let isub_name = (\<lambda>s. s @ isub_of_str name) 
+                            let isub_name = (\<lambda>s. s @ isub_of_str name)
                               ; var_name = name in
                              Expr_basic [isub_name datatype_constr_name, var_oid, var_name])
        ; case_branch = (\<lambda>pat res. (Expr_apply (isub_h datatype_in) [pat], finish_with_some1 res)) in
@@ -432,7 +432,7 @@ definition "print_istypeof_class =
   map_class_gen_h' (\<lambda>isub_name name l_hierarchy.
     map
       (\<lambda> (h_name, l_attr).
-        Defs_overloaded 
+        Defs_overloaded
           (concat (isub_name const_oclistypeof # ''_'' # h_name # []))
           (let var_x = ''x'' in
            Expr_rewrite
@@ -440,18 +440,18 @@ definition "print_istypeof_class =
              unicode_equiv
              (let var_tau = unicode_tau
                 ; ocl_tau = (\<lambda>v. Expr_apply v [Expr_basic [var_tau]]) in
-                Expr_lambda var_tau 
+                Expr_lambda var_tau
                   (Expr_case
                     (ocl_tau var_x)
                     ( (Expr_basic [unicode_bottom], ocl_tau ''invalid'')
                     # (Expr_some (Expr_basic [unicode_bottom]), ocl_tau ''true'')
                     # (let var_oid = wildcard
-                         ; pattern_complex_gen = (\<lambda>f1 f2 h_name name. 
+                         ; pattern_complex_gen = (\<lambda>f1 f2 h_name name.
                             let isub_h = (\<lambda> s. s @ isub_of_str h_name)
-                              ; isub_name = (\<lambda>s. s @ isub_of_str name) 
+                              ; isub_name = (\<lambda>s. s @ isub_of_str name)
                               ; isub_n = (\<lambda>s. isub_name (concat (s # ''_'' # [])))
                               ; var_name = name in
-                             Expr_apply (isub_h datatype_constr_name) 
+                             Expr_apply (isub_h datatype_constr_name)
                                         [Expr_basic [var_oid], Expr_apply (f2 isub_n (isub_h datatype_ext_constr_name)) (f1 var_name)])
                          ; pattern_complex = pattern_complex_gen (\<lambda>x. [Expr_basic [wildcard]]) (\<lambda> f x. f x)
                          ; some_some = (\<lambda>x. Expr_some (Expr_some x)) in
@@ -462,7 +462,7 @@ definition "print_istypeof_class =
                          ret_true (pattern_complex_gen (\<lambda>_. map (\<lambda>_. Expr_basic [wildcard]) l_attr) (\<lambda>_ x. x) name h_name)
                        else if x = Some GT then
                          ret_true (pattern_complex h_name name)
-                       else 
+                       else
                          l_false) ) ))) )
       l_hierarchy)"
 
@@ -473,7 +473,7 @@ definition "print_istypeof_lemmas_id =
 definition "print_istypeof_lemma_cp =
   get_hierarchy (\<lambda>l_hierarchy.
   concat (concat
-  (map (\<lambda>name1. map (\<lambda>name2. map (\<lambda>name3. 
+  (map (\<lambda>name1. map (\<lambda>name2. map (\<lambda>name3.
     Lemma_by
       (concat (''cp_'' # const_oclistypeof # isub_of_str name1 # ''_'' # name3 # ''_'' # name2 # []))
       (bug_ocaml_extraction (let var_p = ''p''; var_x = ''x'' in
@@ -492,14 +492,14 @@ definition "print_istypeof_lemmas_cp =
   get_hierarchy (\<lambda>l_hierarchy.
     [Lemmas_simp
   (concat (concat
-  (map (\<lambda>name1. map (\<lambda>name2. map (\<lambda>name3. 
+  (map (\<lambda>name1. map (\<lambda>name2. map (\<lambda>name3.
       (concat (''cp_'' # const_oclistypeof # isub_of_str name1 # ''_'' # name3 # ''_'' # name2 # []))
   ) l_hierarchy) l_hierarchy) l_hierarchy)))])"
 
 definition "print_istypeof_lemma_strict =
   get_hierarchy (\<lambda>l_hierarchy.
   concat (concat
-  (map (\<lambda>name1. map (\<lambda>(name2,name2'). map (\<lambda>name3. 
+  (map (\<lambda>name1. map (\<lambda>(name2,name2'). map (\<lambda>name3.
     Lemma_by
       (concat (const_oclistypeof # isub_of_str name1 # ''_'' # name3 # ''_'' # name2 # []))
       [ Expr_rewrite
@@ -519,7 +519,7 @@ definition "print_istypeof_lemmas_strict =
   get_hierarchy (\<lambda>l_hierarchy.
   [ Lemmas_simp
   (concat (concat
-  (map (\<lambda>name1. map (\<lambda>name2. map (\<lambda>name3. 
+  (map (\<lambda>name1. map (\<lambda>name2. map (\<lambda>name3.
       (concat (const_oclistypeof # isub_of_str name1 # ''_'' # name3 # ''_'' # name2 # []))
   ) l_hierarchy) [''invalid'',''null'']) l_hierarchy)))])"
 
@@ -530,28 +530,28 @@ definition "print_iskindof_consts =
     Consts (isub_name const_ocliskindof) ty_boolean dot_ocliskindof name)"
 
 definition "print_iskindof_from_universe =
-  map_class_h (\<lambda>isub_name name l_hierarchy. 
+  map_class_h (\<lambda>isub_name name l_hierarchy.
     let const_iskindof = concat (const_ocliskindof # isub_of_str name # ''_'' # unicode_AA # [])
       ; var_u = ''u'' in
-    Definition (Expr_rewrite (Expr_basic [const_iskindof]) ''='' (Expr_lambda var_u 
+    Definition (Expr_rewrite (Expr_basic [const_iskindof]) ''='' (Expr_lambda var_u
 
-   (let ((finish_with_some1, finish_with_some2), last_case_none) = 
+   (let ((finish_with_some1, finish_with_some2), last_case_none) =
      let (f, r) = (if hd l_hierarchy = name then (id, []) else (flip, [(Expr_basic [wildcard], Expr_basic [''None''])])) in
      (f (id, Expr_some), r) in
    finish_with_some2
-   (Expr_case (Expr_basic [var_u]) (concat (map 
-   (\<lambda>h_name. 
+   (Expr_case (Expr_basic [var_u]) (concat (map
+   (\<lambda>h_name.
      let isub_h = (\<lambda> s. s @ isub_of_str h_name)
        ; var_oid = ''oid''
-       ; pattern_complex = (\<lambda>h_name name. 
+       ; pattern_complex = (\<lambda>h_name name.
                             let isub_h = (\<lambda> s. s @ isub_of_str h_name)
-                              ; isub_name = (\<lambda>s. s @ isub_of_str name) 
+                              ; isub_name = (\<lambda>s. s @ isub_of_str name)
                               ; isub_n = (\<lambda>s. isub_name (concat (s # ''_'' # [])))
                               ; var_name = name in
-                             Expr_apply (isub_h datatype_constr_name) 
+                             Expr_apply (isub_h datatype_constr_name)
                                         [Expr_basic [var_oid], Expr_apply (isub_n (isub_h datatype_ext_constr_name)) [Expr_basic [var_name]]])
        ; pattern_simple = (\<lambda> name.
-                            let isub_name = (\<lambda>s. s @ isub_of_str name) 
+                            let isub_name = (\<lambda>s. s @ isub_of_str name)
                               ; var_name = name in
                              Expr_basic [isub_name datatype_constr_name, var_oid, var_name])
        ; case_branch = (\<lambda>pat res. (Expr_apply (isub_h datatype_in) [pat], finish_with_some1 res)) in
@@ -568,7 +568,7 @@ fun print_iskindof_class_aux where
    v @
    (let isub_name = (\<lambda>s. s @ isub_of_str name) in
    map (\<lambda> h_name.
-    Defs_overloaded 
+    Defs_overloaded
           (concat (isub_name const_ocliskindof # ''_'' # h_name # []))
           (let var_x = ''x'' in
            Expr_rewrite
@@ -588,7 +588,7 @@ definition "print_iskindof_lemmas_id =
 definition "print_iskindof_lemma_cp =
   get_hierarchy (\<lambda>l_hierarchy.
   concat (concat
-  (map (\<lambda>name1. map (\<lambda>name2. map (\<lambda>name3. 
+  (map (\<lambda>name1. map (\<lambda>name2. map (\<lambda>name3.
     Lemma_by
       (concat (''cp_'' # const_ocliskindof # isub_of_str name1 # ''_'' # name3 # ''_'' # name2 # []))
       (bug_ocaml_extraction (let var_p = ''p''; var_x = ''x'' in
@@ -607,14 +607,14 @@ definition "print_iskindof_lemmas_cp =
   get_hierarchy (\<lambda>l_hierarchy.
     [Lemmas_simp
   (concat (concat
-  (map (\<lambda>name1. map (\<lambda>name2. map (\<lambda>name3. 
+  (map (\<lambda>name1. map (\<lambda>name2. map (\<lambda>name3.
       (concat (''cp_'' # const_ocliskindof # isub_of_str name1 # ''_'' # name3 # ''_'' # name2 # []))
   ) l_hierarchy) l_hierarchy) l_hierarchy)))])"
 
 definition "print_iskindof_lemma_strict =
   get_hierarchy (\<lambda>l_hierarchy.
   concat (concat
-  (map (\<lambda>name1. map (\<lambda>(name2,name2'). map (\<lambda>name3. 
+  (map (\<lambda>name1. map (\<lambda>(name2,name2'). map (\<lambda>name3.
     Lemma_by
       (concat (const_ocliskindof # isub_of_str name1 # ''_'' # name3 # ''_'' # name2 # []))
       [ Expr_rewrite
@@ -634,7 +634,7 @@ definition "print_iskindof_lemmas_strict =
   get_hierarchy (\<lambda>l_hierarchy.
   [ Lemmas_simp
   (concat (concat
-  (map (\<lambda>name1. map (\<lambda>name2. map (\<lambda>name3. 
+  (map (\<lambda>name1. map (\<lambda>name2. map (\<lambda>name3.
       (concat (const_ocliskindof # isub_of_str name1 # ''_'' # name3 # ''_'' # name2 # []))
   ) l_hierarchy) [''invalid'',''null'']) l_hierarchy)))])"
 
@@ -681,7 +681,7 @@ definition "print_select =
     let var_f = ''f''
       ; wildc = Expr_basic [wildcard] in
     let (_, _, l) = (foldl
-      (\<lambda>(l_wildl, l_wildr, l_acc) (attr, _). 
+      (\<lambda>(l_wildl, l_wildr, l_acc) (attr, _).
         let isup_attr = (\<lambda>s. s @ isup_of_str attr) in
         ( wildc # l_wildl
         , tl l_wildr
@@ -689,7 +689,7 @@ definition "print_select =
                        (Expr_basic [isup_attr (isub_name var_select), var_f])
                        ''=''
                        (let var_x = ''x''
-                          ; var_attr = attr in 
+                          ; var_attr = attr in
                         Expr_lambda
                           var_x
                           (Expr_case
@@ -702,7 +702,7 @@ definition "print_select =
                                                        , rhs))
                               [ ( Expr_basic [unicode_bottom], Expr_basic [''null''] )
                               , ( Expr_some (Expr_basic [var_attr])
-                                , Expr_apply var_f [ bug_ocaml_extraction 
+                                , Expr_apply var_f [ bug_ocaml_extraction
                                                      (let var_x = ''x'' in
                                                         Expr_lambdas [var_x, wildcard] (Expr_some (Expr_some (Expr_basic [var_x]))))
                                                    , Expr_basic [var_attr]]) ]) # [(wildc, Expr_basic [''invalid''])] # []))))) # l_acc))
@@ -732,5 +732,228 @@ definition "print_dot =
           l_attr)
         [ (var_in_post_state, '''', '''')
         , (var_in_pre_state, ''_at_pre'', ''@pre'')])))"
+
+subsection{* OCaml *}
+type_synonym sl = String.literal
+
+subsubsection{* module Printf *}
+
+consts sprintf0 :: "sl \<Rightarrow> sl"
+consts sprintf1 :: "sl \<Rightarrow> '\<alpha>1 \<Rightarrow> sl"
+consts sprintf2 :: "sl \<Rightarrow> '\<alpha>1 \<Rightarrow> '\<alpha>2 \<Rightarrow> sl"
+consts sprintf3 :: "sl \<Rightarrow> '\<alpha>1 \<Rightarrow> '\<alpha>2 \<Rightarrow> '\<alpha>3 \<Rightarrow> sl"
+consts sprintf4 :: "sl \<Rightarrow> '\<alpha>1 \<Rightarrow> '\<alpha>2 \<Rightarrow> '\<alpha>3 \<Rightarrow> '\<alpha>4 \<Rightarrow> sl"
+consts sprintf5 :: "sl \<Rightarrow> '\<alpha>1 \<Rightarrow> '\<alpha>2 \<Rightarrow> '\<alpha>3 \<Rightarrow> '\<alpha>4 \<Rightarrow> '\<alpha>5 \<Rightarrow> sl"
+consts sprintf6 :: "sl \<Rightarrow> '\<alpha>1 \<Rightarrow> '\<alpha>2 \<Rightarrow> '\<alpha>3 \<Rightarrow> '\<alpha>4 \<Rightarrow> '\<alpha>5 \<Rightarrow> '\<alpha>6 \<Rightarrow> sl"
+
+code_const sprintf0 (OCaml "Printf.sprintf")
+code_const sprintf1 (OCaml "Printf.sprintf")
+code_const sprintf2 (OCaml "Printf.sprintf")
+code_const sprintf3 (OCaml "Printf.sprintf")
+code_const sprintf4 (OCaml "Printf.sprintf")
+code_const sprintf5 (OCaml "Printf.sprintf")
+code_const sprintf6 (OCaml "Printf.sprintf")
+
+consts eprintf0 :: "sl \<Rightarrow> unit"
+code_const eprintf0 (OCaml "Printf.eprintf")
+
+subsubsection{* module String *}
+
+consts String_concat :: "sl \<Rightarrow> sl list \<Rightarrow> sl"
+code_const String_concat (OCaml "String.concat")
+
+subsubsection{* module List *}
+
+definition "List_iter f l = foldl (\<lambda>_. f) () l"
+definition "List_flatten l = foldl (\<lambda>acc l. foldl (\<lambda>acc x. x # acc) acc (rev l)) [] (rev l)"
+definition "List_mapi f l = (let (l, _) = foldl (\<lambda>(acc, n) x. (f n x # acc, Suc n)) ([], 0) l in rev l)"
+
+subsubsection{* beginning *}
+
+code_include OCaml "" {*
+
+module Variant = struct
+  type nat = [ `ZeroNat | `Suc of nat ]
+
+  type nibble = [ `Nibble0 | `Nibble1 | `Nibble2 | `Nibble3 | `Nibble4 | `Nibble5 |
+    `Nibble6 | `Nibble7 | `Nibble8 | `Nibble9 | `NibbleA | `NibbleB | `NibbleC | `NibbleD
+    | `NibbleE | `NibbleF ]
+
+  type char = [ `Char of nibble * nibble ]
+end
+
+module To = struct
+  module M = struct
+    let to_n = function
+      `Nibble0 -> 0x0 | `Nibble1 -> 0x1 | `Nibble2 -> 0x2 | `Nibble3 -> 0x3 | `Nibble4 -> 0x4 | `Nibble5 -> 0x5 |
+       `Nibble6 -> 0x6 | `Nibble7 -> 0x7 | `Nibble8 -> 0x8 | `Nibble9 -> 0x9 | `NibbleA -> 0xA | `NibbleB -> 0xB | `NibbleC -> 0xC | `NibbleD -> 0xD
+      | `NibbleE -> 0xE | `NibbleF -> 0xF
+
+    let to_c = function `Char (n1, n2) -> char_of_int (to_n n1 lsl 4 + to_n n2)
+
+    let to_s l = (String.concat "" (List.map (fun c -> String.make 1 (to_c c)) l))
+  (*
+    let to_num =
+      let rec aux mot n = function
+        | `Bit0 p -> aux mot (succ n) p
+        | bit ->
+          let mot = mot + (1 lsl n) in
+          match bit with
+          | `Bit1 p -> aux mot (succ n) p
+          | _ -> mot in
+      aux 0 0
+
+    let to_i = function
+      | `ZeroInt -> 0
+      | `Pos n -> to_num n
+      | `Neg n -> - (to_num n)
+  *)
+    let rec to_nat = function `ZeroNat -> 0 | `Suc n -> succ (to_nat n)
+  end
+  let s = M.to_s
+  let n = M.to_nat
+end
+
+module Escape = struct
+  (* here contain functions using the '_' character
+     (that is not allowed in a Isabelle 'code_const' expr) *)
+
+  module Sys = struct open Sys
+    let fileExists = file_exists
+    let isDirectory = is_directory
+  end
+
+  module Pervasives = struct
+    let openOut = open_out
+    let closeOut = close_out
+  end
+
+  let comp f g x = f (g x)
+  let forget g _ = g
+  let err = Printf.eprintf "File exists %s\n"
+end
+
+*}
+
+consts out_file0 :: "((sl \<Rightarrow> unit) (* fprintf *) \<Rightarrow> unit) \<Rightarrow> sl \<Rightarrow> unit"
+consts out_file1 :: "((sl \<Rightarrow> '\<alpha>1 \<Rightarrow> unit) (* fprintf *) \<Rightarrow> unit) \<Rightarrow> sl \<Rightarrow> unit"
+code_const out_file1 (OCaml "(fun f file ->
+  let () = if Escape.Sys.fileExists file then Escape.err file else () in
+  let oc = Escape.Pervasives.openOut file in
+  let () = f (Printf.fprintf oc) in
+  Escape.Pervasives.closeOut oc)")
+
+definition "escapeNatRec = nat_rec" 
+
+consts To_s :: "string \<Rightarrow> sl"
+code_const To_s (OCaml "(fun s ->
+  let ofN = function
+    Nibble0 -> `Nibble0 | Nibble1 -> `Nibble1 | Nibble2 -> `Nibble2 | Nibble3 -> `Nibble3 | Nibble4 -> `Nibble4 | Nibble5 -> `Nibble5 |
+    Nibble6 -> `Nibble6 | Nibble7 -> `Nibble7 | Nibble8 -> `Nibble8 | Nibble9 -> `Nibble9 | NibbleA -> `NibbleA | NibbleB -> `NibbleB |
+    NibbleC -> `NibbleC | NibbleD -> `NibbleD | NibbleE -> `NibbleE | NibbleF -> `NibbleF in
+  let ofC = function Char (c1, c2) -> `Char (ofN c1, ofN c2) in
+  To.s (List.map ofC s))")
+
+consts To_i :: "nat \<Rightarrow> sl"
+code_const To_i (OCaml "(let (<<) = Escape.comp in
+  To.n (* REMARK [Obj.magic] ? *) << escapeNatRec `ZeroNat (Escape.forget (fun x -> `Suc x)))")
+
+subsubsection{* module Sys *}
+
+consts Sys_is_directory :: "sl \<Rightarrow> bool"
+code_const Sys_is_directory (OCaml "Escape.Sys.isDirectory")
+
+subsubsection{* module Unicode *}
+
+definition "Unicode_mk_u = sprintf1 (STR (Char Nibble5 NibbleC # ''<%s>''))"
+definition "Unicode_u_Rightarrow = Unicode_mk_u (STR ''Rightarrow'')"
+definition "Unicode_u_alpha = Unicode_mk_u (STR ''alpha'')"
+definition "Unicode_u_lambda = Unicode_mk_u (STR ''lambda'')"
+definition "Unicode_u_lfloor = Unicode_mk_u (STR ''lfloor'')"
+definition "Unicode_u_rfloor = Unicode_mk_u (STR ''rfloor'')"
+definition "Unicode_u_Longrightarrow = Unicode_mk_u (STR ''Longrightarrow'')"
+
+subsubsection{* module s_of *}
+
+definition "s_of_datatype = (\<lambda> Datatype n l \<Rightarrow>
+  sprintf2 (STR ''datatype %s = %s'')
+    (To_s n)
+    (String_concat (STR ''
+                        | '')
+      (map
+        (\<lambda>(n,l).
+         sprintf2 (STR ''%s %s'')
+           (To_s n)
+           (String_concat (STR '' '')
+            (map
+              (\<lambda> Opt o_ \<Rightarrow> sprintf1 (STR ''\"%s option\"'') (To_s o_)
+               | Raw o_ \<Rightarrow> sprintf1 (STR ''%s'') (To_s o_))
+              l))) l) ))"
+
+fun s_of_rawty where "s_of_rawty rawty = (case rawty of
+    Ty_base s \<Rightarrow> To_s s
+  | Ty_apply name l \<Rightarrow> sprintf2 (STR ''%s %s'') (let s = String_concat (STR '', '') (map s_of_rawty l) in
+                                                 case l of [_] \<Rightarrow> s | _ \<Rightarrow> sprintf1 (STR ''(%s)'') s)
+                                                (s_of_rawty name))"
+
+definition "s_of_tsynonym = (\<lambda> Type_synonym n l \<Rightarrow> 
+    sprintf2 (STR ''type_synonym %s = \"%s\"'') (To_s n) (s_of_rawty l))"
+
+fun s_of_expr where "s_of_expr expr = (case expr of
+    Expr_case e l \<Rightarrow> sprintf2 (STR ''(case %s of %s)'') (s_of_expr e) (String_concat (STR ''
+    | '') (map (\<lambda> (s1, s2) \<Rightarrow> sprintf3 (STR ''%s %s %s'') (s_of_expr s1) Unicode_u_Rightarrow (s_of_expr s2)) l))
+  | Expr_rewrite e1 symb e2 \<Rightarrow> sprintf3 (STR ''%s %s %s'') (s_of_expr e1) (To_s symb) (s_of_expr e2)
+  | Expr_basic l \<Rightarrow> sprintf1 (STR ''%s'') (String_concat (STR '' '') (map To_s l))
+  | Expr_binop e1 s e2 \<Rightarrow> sprintf3 (STR ''%s %s %s'') (s_of_expr e1) (s_of_expr (Expr_basic [s])) (s_of_expr e2)
+  | Expr_annot e s \<Rightarrow> sprintf2 (STR ''(%s::%s)'') (s_of_expr e) (To_s s)
+  | Expr_lambda s e \<Rightarrow> sprintf3 (STR ''(%s%s. %s)'') Unicode_u_lambda (To_s s) (s_of_expr e)
+  | Expr_lambdas l e \<Rightarrow> sprintf3 (STR ''(%s%s. %s)'') Unicode_u_lambda (String_concat (STR '' '') (map To_s l)) (s_of_expr e)
+  (*| Expr_apply s [e] \<Rightarrow> sprintf2 (STR ''(%s %s)'') (To_s s) (s_of_expr e)*)
+  | Expr_apply s l \<Rightarrow> sprintf2 (STR ''(%s %s)'') (To_s s) (String_concat (STR '' '') (map (\<lambda> e \<Rightarrow> sprintf1 (STR ''(%s)'') (s_of_expr e)) l))
+  | Expr_some e \<Rightarrow> sprintf3 (STR ''%s%s%s'') Unicode_u_lfloor (s_of_expr e) Unicode_u_rfloor
+  | Expr_postunary e1 e2 \<Rightarrow> sprintf2 (STR ''%s %s'') (s_of_expr e1) (s_of_expr e2)
+  | Expr_warning_parenthesis e \<Rightarrow> sprintf1 (STR ''(%s)'') (s_of_expr e)
+  | Expr_parenthesis e \<Rightarrow> sprintf1 (STR ''(%s)'') (s_of_expr e))"
+
+definition "s_of_instantiation = (\<lambda> Instantiation n n_def expr \<Rightarrow>
+    let name = To_s n in
+    sprintf4 (STR ''instantiation %s :: object
+begin
+  definition %s_%s_def : \"%s\"
+  instance ..
+end'')
+      name
+      (To_s n_def)
+      name
+      (s_of_expr expr))"
+
+definition "s_of_defs_overloaded = (\<lambda> Defs_overloaded n e \<Rightarrow>
+    sprintf2 (STR ''defs(overloaded) %s : \"%s\"'') (To_s n) (s_of_expr e))"
+
+definition "s_of_consts_class = (\<lambda> Consts n ty_out symb1 symb2 \<Rightarrow>
+    sprintf6 (STR ''consts %s :: \"'%s %s %s\" (\"(_) %s'(%s')\")'') (To_s n) Unicode_u_alpha Unicode_u_Rightarrow (To_s ty_out) (To_s symb1) (To_s symb2))"
+
+definition "s_of_definition_hol = (\<lambda>
+    Definition e \<Rightarrow> sprintf1 (STR ''definition \"%s\"'') (s_of_expr e)
+  | Definition_abbrev name (abbrev, prio) e \<Rightarrow> sprintf4 (STR ''definition %s (\"(1%s)\" %d)
+  where \"%s\"'') (To_s name) (s_of_expr abbrev) (To_i prio) (s_of_expr e))"
+
+definition "s_of_lemmas_simp = (\<lambda> Lemmas_simp l \<Rightarrow>
+    sprintf1 (STR ''lemmas [simp] = %s'') (String_concat (STR ''
+                '') (map (To_s) l)))"
+
+definition "s_of_tactic = (\<lambda>
+    Tac_rule s \<Rightarrow> sprintf1 (STR ''rule %s'') (To_s s)
+  | Tac_simp \<Rightarrow> sprintf0 (STR ''simp'')
+  | Tac_simp_add l \<Rightarrow> sprintf1 (STR ''simp add: %s'') (String_concat (STR '' '') (map To_s l))
+  | Tac_simp_all \<Rightarrow> sprintf0 (STR ''simp_all'')
+  | Tac_simp_all_add s \<Rightarrow> sprintf1 (STR ''simp_all add: %s'') (To_s s))"
+
+definition "s_of_lemma_by = (\<lambda> Lemma_by n l_spec l_apply \<Rightarrow>
+    sprintf3 (STR ''lemma %s : \"%s\"
+by(%s)'')
+      (To_s n)
+      (String_concat (sprintf1 (STR '' %s '') Unicode_u_Longrightarrow) (map s_of_expr l_spec))
+      (String_concat (STR '', '') (map s_of_tactic l_apply)))"
 
 end
